reflex/coq/bench-quark/PolicyAddressBarCorrectnessNewTabEnables.v
@@ -1,0 +1,27 @@
+Require Import String.
+Require Import Reflex ReflexBase.
+Require Import PolLang ActionMatch.
+Require Import Kernel.
+
+Local Opaque str_of_string.
+
+Import SystemFeatures Language Spec.
+
+Definition UserInput_pat : conc_pat COMPT COMPS :=
+  Build_conc_pat COMPT COMPS UserInput tt.
+
+Definition Tab_pat id d : conc_pat COMPT COMPS :=
+  Build_conc_pat COMPT COMPS Tab (Some id, (Some d, tt)).
+
+Theorem enables : forall st tr id d,
+  Reach PAYD COMPT COMPTDEC COMPS KSTD IENVD INIT HANDLERS st ->
+  ktr _ _ _ _ st = inhabits tr ->
+  Enables PAYD COMPT COMPS COMPTDEC
+    (KOExec PAYD COMPT COMPS None None (Some (Tab_pat id d)))
+    (KOSend PAYD COMPT COMPS (Some UserInput_pat)
+      (Some (Build_opt_msg PAYD
+        AddrAdd (Some id, (Some d, tt)))))
+          tr.
+Proof.
+  Time solve [crush].
+Time Qed.
