reflex/coq/bench-quark/PolicyAddressBarCorrectnessSwitch.v
@@ -1,0 +1,30 @@
+Require Import String.
+Require Import Reflex ReflexBase.
+Require Import PolLang ActionMatch.
+Require Import Kernel.
+
+Local Opaque str_of_string.
+
+Import SystemFeatures Language Spec.
+
+Definition UserInput_pat : conc_pat COMPT COMPS :=
+  Build_conc_pat COMPT COMPS UserInput tt.
+
+Definition Output_pat : conc_pat COMPT COMPS :=
+  Build_conc_pat COMPT COMPS Output tt.
+
+Theorem imm_after : forall st tr id,
+  Reach PAYD COMPT COMPTDEC COMPS KSTD IENVD INIT HANDLERS st ->
+  ktr _ _ _ _ st = inhabits tr ->
+  ImmAfter PAYD COMPT COMPS COMPTDEC
+    (KOSend PAYD COMPT COMPS (Some (Output_pat))
+            (Some (Build_opt_msg PAYD
+                                RenderCompleted (Some id, tt))))
+    (KOSend PAYD COMPT COMPS (Some (UserInput_pat))
+            (Some (Build_opt_msg PAYD
+                                AddrFocus (Some id, tt))))
+    tr.
+Proof.
+  crush. unfold Reflex.match_comp, Reflex.match_comp_pf in *. simpl in *.
+  Time solve [crush].
+Time Qed.
